Extend Spec.ECIES module

specs/Spec.ECIES.fst
@@ -86,7 +86,7 @@ val encap:
   -> e: entropy
   -> pk: key_public_s cs
   -> context: lbytes 32 ->
-  Tot (entropy & (option (key_s cs & key_private_s cs & key_public_s cs)))
+  Tot (entropy & (option (key_s cs & key_public_s cs)))
 
 let encap cs e pk context =
   let e', esk = crypto_random e (size_key_dh cs) in
@@ -98,7 +98,7 @@ let encap cs e pk context =
     let extracted = HKDF.hkdf_extract (hash_of_cs cs) salt secret in
     let info = (id_of_cs cs) @| const_label_key @| context in
     let key = HKDF.hkdf_expand (hash_of_cs cs) extracted info (size_key cs) in
-    e', Some (key, esk, epk)
+    e', Some (key, epk)
 
 
 val decap:
@@ -154,3 +154,46 @@ let decrypt cs sk input aad counter =
   let nonce = sub sk klen (size_nonce cs - numbytes U32) in
   let ctr = uint_to_bytes_le counter in
   AEAD.aead_decrypt (aead_of_cs cs) key (nonce @| ctr) input aad
+
+///
+/// One time KEM API
+///
+
+(** KEM Encrypt a payload to a specific Group or Participant *)
+val encrypt_single:
+    cs: ciphersuite
+  -> e: entropy
+  -> pk: key_public_s cs
+  -> input: bytes{length input <= max_size_t
+           /\ length input + size_key_dh cs + AEAD.size_block (aead_of_cs cs) <= max_size_t
+           /\ length input + size_key_dh cs + AEAD.padlen (aead_of_cs cs) (length input) <= max_size_t}
+  -> context: lbytes 32 ->
+  Tot (entropy & (option (lbytes (size_key_dh cs + length input + AEAD.size_tag (aead_of_cs cs)))))
+
+let encrypt_single cs e pk input context =
+  match encap cs e pk context with
+  | e', None -> e', None
+  | e', Some (key, epk) ->
+    let ciphertext = encrypt cs key input lbytes_empty (u32 0) in
+    e', Some (concat #uint8 #(size_key_dh cs) #(length input + AEAD.size_tag (aead_of_cs cs)) epk ciphertext)
+
+
+(** KEM Decrypt a payload that was generated using KEM Encrypt *)
+val decrypt_single:
+    cs: ciphersuite
+  -> sk: key_private_s cs
+  -> epk: key_public_s cs
+  -> input: bytes {size_key_dh cs + AEAD.size_tag (aead_of_cs cs) <= length input /\ length input <= max_size_t}
+  -> context: lbytes 32 ->
+  Tot (option (lbytes (length input - AEAD.size_tag ((aead_of_cs cs)))))
+
+let decrypt_single cs sk epk input context =
+  let epk = sub #uint8 #(length input) input 0 (size_key_dh cs) in
+  let ciphertext = sub #uint8 #(length input) input (size_key_dh cs) ((length input) - size_key_dh cs) in
+  match decap cs sk epk context with
+  | None -> None
+  | Some key ->
+    match decrypt cs key ciphertext lbytes_empty (u32 0) with
+    | None -> None
+    | Some plaintext ->
+      Some (concat #uint8 #(size_key_dh cs) #(length input - (size_key_dh cs) - AEAD.size_tag (aead_of_cs cs)) epk plaintext)
